Remove logic reflexivity and simplify

type_system/subtyping_lemmas.v
@@ -413,14 +413,13 @@ inv r. eapply Respects; auto. destruct H3.
 intros wf ctxsty.
 inv equals. destruct H3; apply Veq; eauto.
 all: clear ctx_subtype_vtype ctx_subtype_ctype ctx_subtype_htype.
-+ apply VeqRefl. auto.
 + apply VeqSym. eauto.
 + eapply VeqTrans; eauto.
 + eapply ctx_subtype_get_rev in ctxsty as cget; eauto.
   destruct cget as [A''[gets sty]]. 
   eapply VeqVar; eauto. eapply vsubtype_trans; eauto.
 + eapply VeqUnit.
-+ eapply VeqInt. auto.
++ eapply VeqInt.
 + eapply VeqPair; eauto.
 + eapply VeqInl; eauto.
 + eapply VeqInr; eauto.
@@ -437,7 +436,6 @@ all: clear ctx_subtype_vtype ctx_subtype_ctype ctx_subtype_htype.
 intros wf ctxsty.
 inv equals. destruct H3; apply Ceq; eauto.
 all: clear ctx_subtype_vtype ctx_subtype_ctype ctx_subtype_htype ctx_subtype_heq.
-+ apply CeqRefl. auto.
 + apply CeqSym. eauto.
 + eapply CeqTrans; eauto.
 + eapply CeqRet; eauto.
@@ -483,7 +481,6 @@ all: clear ctx_subtype_vtype ctx_subtype_ctype ctx_subtype_htype ctx_subtype_heq
 intros wf ctxsty.
 inv equals. destruct H4; apply Heq; eauto.
 all: clear ctx_subtype_vtype ctx_subtype_ctype ctx_subtype_htype.
-+ apply HeqRefl. auto.
 + apply HeqSym. eauto.
 + eapply HeqTrans; eauto.
 + eapply HeqSigØ.
@@ -495,106 +492,6 @@ all: clear ctx_subtype_vtype ctx_subtype_ctype ctx_subtype_htype.
     apply vsubtype_refl. inv H. assumption.
 }
 Qed.
-
-
-(* ==================== Logic Subtyping ==================== *)
-
-Fixpoint veq_subtype A A' Γ v1 v2 (orig : veq A Γ v1 v2) {struct orig} :
-  wf_vtype A' -> vsubtype A A' -> veq A' Γ v1 v2
-
-with ceq_subtype C C' Γ c1 c2 (orig : ceq C Γ c1 c2) {struct orig} :
-  wf_ctype C' -> csubtype C C' -> ceq C' Γ c1 c2
-
-with heq_subtype Σ Σ' D D' Γ h1 h2 (orig : heq Σ D Γ h1 h2) {struct orig} :
-  wf_sig Σ' -> wf_ctype D' -> sig_subtype Σ' Σ -> csubtype D D' -> 
-  heq Σ' D' Γ h1 h2.
-
-Proof.
-{ 
-intros. inv orig.
-assert (has_vtype Γ v1 A') as ty1.
-{ apply TypeV; auto. eapply TypeVSubtype; eauto. }
-assert (has_vtype Γ v2 A') as ty2.
-{ apply TypeV; auto. eapply TypeVSubtype; eauto. }
-induction H5; apply Veq; auto.
-+ apply VeqRefl. auto.
-+ apply VeqSym. eauto.
-+ eapply VeqTrans; eauto.
-+ eapply VeqVar; eauto. eapply vsubtype_trans; eauto.
-+ inv H0. apply VeqUnit; eauto.
-+ inv H0. apply VeqInt; eauto.
-+ inv H0. inv H. eapply VeqPair; eapply veq_subtype; eauto.
-+ inv H0. eapply VeqInl. eapply veq_subtype; eauto. inv H. auto.
-+ inv H0. eapply VeqInr. eapply veq_subtype; eauto. inv H. auto.
-+ inv H0. apply VeqFun. inv H. eapply ceq_subtype in H5; eauto.
-  eapply ctx_subtype_ceq. eauto.
-  - apply WfCtxU; auto.
-  - apply SubtypeCtxU; auto. apply ctx_subtype_refl. auto.
-+ inv H0. inv H9. apply VeqHandler. eapply ceq_subtype in H5; eauto.
-  eapply ctx_subtype_ceq. eauto. all: inv H.
-  - apply WfCtxU; auto. inv H8.  assumption.
-  - apply SubtypeCtxU; auto. apply ctx_subtype_refl. auto.
-  - assumption.
-  - eapply heq_subtype. eauto. inv H8. all: assumption.
-+ inv H0. apply ηUnit.
-+ inv H0. apply ηFun.
-}{
-intros. inv orig. 
-assert (has_ctype Γ c1 C') as ty1.
-{ apply TypeC; auto. eapply TypeCSubtype; eauto. }
-assert (has_ctype Γ c2 C') as ty2.
-{ apply TypeC; auto. eapply TypeCSubtype; eauto. }
-apply Ceq; auto. destruct H5.
-+ apply CeqRefl. auto.
-+ apply CeqSym. eauto.
-+ eapply CeqTrans; eauto.
-+ inv H0. inv H. eapply CeqRet; eauto.
-+ eapply CeqAbsurd; eauto.
-+ eapply CeqΠMatch; eauto.
-+ eapply CeqΣMatch; eauto.
-+ eapply CeqDoBind; eauto.
-+ eapply CeqApp; eauto. eapply veq_subtype; eauto; inv H5; inv H7.
-  - apply WfTyFun; assumption.
-  - apply SubtypeTyFun. apply vsubtype_refl. all: auto.
-+ eapply CeqHandle; eauto. eapply veq_subtype; eauto; inv H5; inv H7.
-  - apply WfTyHandler; assumption.
-  - apply SubtypeTyHandler. apply csubtype_refl. all: auto.
-+ eapply CeqLetRec; eauto.
-+ inv H0. eapply sig_subtype_get_Some in H5; eauto.
-  destruct H5 as [A_op'[B_op'[gets[asty bsty]]]].
-  eapply CeqOp; eauto.
-  - eapply veq_subtype; eauto.
-    eapply get_op_type_wf in gets. destruct gets. auto.
-    inv H. auto.
-  - eapply ctx_subtype_ceq; eauto.
-    * eapply ceq_subtype; eauto. apply SubtypeCTy; auto.
-    * apply WfCtxU. auto. 
-      eapply get_op_type_wf in gets. destruct gets. auto.
-      inv H. auto.
-    * eapply SubtypeCtxU. apply ctx_subtype_refl. all: auto.
-+ eapply βΠMatch.
-+ eapply βΣMatch_Inl.
-+ eapply βΣMatch_Inr.
-+ eapply βApp.
-+ eapply βLetRec.
-+ eapply βDoBind_Ret.
-+ eapply βDoBind_Op.
-+ eapply βHandle_Ret.
-+ eapply βHandle_Op. eauto.
-}{
-intros. inv orig.
-assert (has_htype Γ h1 Σ' D') as ty1.
-{ admit. }
-assert (has_htype Γ h2 Σ' D') as ty2.
-{ admit. } 
-apply Heq; auto. destruct H8.
-+ apply HeqRefl. auto.
-+ apply HeqSym. eauto.
-+ eapply HeqTrans; eauto.
-+ inv H1. eapply HeqSigØ. simpl in H7. discriminate.
-+ inv H1. eapply HeqSigØ. eapply HeqSigU. all: admit.  
-}
-Admitted.
 
 
 (* ==================== Subtype Shapes ==================== *)
